src/FO.v
@@ -1,0 +1,674 @@
+Require Import Common. 
+Require Import DList. 
+Require Import Core. 
+
+  
+  (**  The compilation function itself *)
+  (* exec : forall t (pointer : R t) (guard : expr R Bool) (effects : list effect), block t *)
+  Definition compile (varunit : R Unit) t (a : action Phi R t) : ( block ). 
+  refine (
+      let compile := fix compile t (a  : action Phi R t ) {struct a}  :
+                   (R t -> expr R Bool -> list effect -> block) -> block  :=  
+          match a with 
+            | Return t exp => _
+            | Bind t u A F => _
+            | Assert exp => _
+            | Primitive args res p exprs => _
+            | Try A => _
+          end
+      in _
+    ). 
+  (* return *)
+  intros cont. 
+  refine (binding _  (bind_expr _ exp) (fun X => (cont X (#b true) nil))). 
+  (* bind *)
+  intros cont. 
+  refine (compile _ A  (fun pointerA guardA effectA => 
+                           let B := F pointerA in 
+                             compile _ B  (fun pointerB guardB effectB => 
+                                              cont pointerB (andb guardA guardB) (List.app effectA effectB)
+                                           )
+                                                    
+         )). 
+  (* assert *)
+  intros cont. 
+  refine (binding _  (bind_expr _ exp) (fun X => cont varunit (!X)%expr nil)).   
+  (* primitive *)
+  revert exprs. 
+  refine (match p with
+            | register_read t v => _
+            | register_write t v => _
+            | regfile_read n t v p => _
+            | regfile_write n t v p => _
+          end); clear p; intros exprs cont.         
+  (* register read *)
+  refine (binding _  (bind_reg_read _ v)
+                   (fun X => cont X (#b true)%expr nil)
+         ). 
+  (* register write *)
+   eapply dlist_fold' in exprs. destruct exprs as [w _]. 
+   refine (
+       binding  _ (bind_expr _ w) 
+               (fun X => 
+                  let effects := ([effect_reg_write _ v X])%list in 
+                  cont varunit (#b true)%expr effects
+               )
+     ). 
+   auto. 
+  (* register file read *)
+  eapply dlist_fold' in exprs. simpl in exprs. destruct exprs as [adr _].  
+  refine (
+      binding _ (bind_expr _ adr) 
+              (fun ADR => 
+                  binding _ (bind_regfile_read _ _ v _ ADR)
+                          (fun V => 
+                             cont V (#b true)%expr nil
+                          )
+              )). 
+  auto. 
+  (* register file write *)
+  eapply dlist_fold' in exprs. simpl in exprs. destruct exprs as [adr [w _]].  
+  refine (
+      binding _ (bind_expr _ adr) (fun ADR => 
+                                       binding _ (bind_expr _ w)
+                                               (fun W => 
+                                                  let effects := ([effect_regfile_write _ _ v _ ADR W])%list in 
+                                                  cont varunit (#b true)%expr  effects
+)
+                                    )
+  ). 
+  auto. 
+  (* try *)
+  intros cont. 
+  refine (
+      let block :=   compile _ A (fun _ guardA effectA => 
+                                      let block := exec guardA effectA  in 
+                                        block
+                                   ) in 
+        
+        cont varunit (#b true) ([effect_block block])%list
+             ). 
+  (* conclusion *)
+  eapply compile. apply a.  
+  intros. eapply exec; auto.  
+Defined. 
+
+End t. 
+
+(** * Semantics *)
+
+Section sem. 
+
+  Variable Phi : state. 
+  Variable st : eval_state Phi. 
+  Notation updates := (eval_env (option ∘ eval_sync) Phi). 
+  Definition eval_bind t (b : bind Phi eval_type t) : option (eval_type t).
+  refine (match b with
+            | bind_expr x => Some (eval_expr _ x)
+            | bind_reg_read v => Some  (get _ _ v st)
+            | bind_regfile_read n v p adr => 
+                let rf := get Phi (Tregfile n t) v st in
+                  Regfile.get rf (Word.unsigned adr)                
+          end
+         ). 
+  Defined. 
+                                    
+  Fixpoint eval_block (a : block Phi eval_type) {struct a}: updates -> option updates :=
+    match a with
+      | binding arg bind cont => 
+          fun Delta => 
+            do res <- eval_bind _ bind;
+            eval_block (cont res) Delta
+      | exec guard effects => 
+        let fix  eval_effects (l : list (effect Phi eval_type)) : updates -> option updates :=
+            match l with 
+                | nil => fun Delta => Some Delta 
+                | cons e q => fun Delta => 
+                    match e with 
+                      | effect_block b => eval_block  b Delta
+                      | effect_reg_write t v w =>                                               
+                          Core.Diff.add Phi Delta (Treg t) v w 
+                      | effect_regfile_write  n t v p adr w  =>  
+                          let rf := get Phi (Tregfile n t) v st in                          
+                          let rf := Regfile.set rf (Word.unsigned adr) w in 
+                            Core.Diff.add Phi Delta (Tregfile n t) v rf            
+                    end 
+            end 
+        in 
+          eval_effects effects
+    end. 
+
+End sem. 
+
+Arguments binding {Phi R arg} _ _.  
+Notation "'DO' X <- E ; F" := (binding E (fun X => F)).  
+Arguments bind_expr  {Phi R t} _%expr. 
+Notation "[: v ]" := (bind_reg_read _ _ _ v).  
+Section test. 
+  Require Import MOD. 
+  Definition Z (t : type) := nat. 
+  Eval compute in compile _ _ 0 _ (iterate 5 Z) . 
+
+  Eval compute in compile _ _ 0 _ (done 5 Z). 
+
+End test. 
+
+Section test2. 
+  Require Import Isa. 
+  Eval compute in compile _ _ 0 _ (loadi_rule 5 (fun _ => nat)). 
+
+  Eval compute in compile _ _ 0 _ (store_rule 5 (fun _ => nat)). 
+
+End test2. 
+
+(**  Each primitive in the top level language has must be massaged in
+smaller blocks whose semantics that depend only on the initial state. 
+
+This is naturally the case for [regs], and register [files]. I added
+[visible] just to make the problem obvious in the following
+translation.  
+
+Consider v a [visible]
+
+[ 
+  do _ <- write [: v <- e];
+  assert P; 
+  do x <- read [: v ];
+  assert Q(x); 
+  A
+]
+
+must be translated to 
+[
+ t1 <- e; 
+ Guard (P /\ Q(t1))
+   [
+    write [: v <- t1]; 
+    x <- t1; 
+    A
+   ]
+] 
+
+The global strategy is as follows:
+- All combinational operations bubble to the top of a block; 
+- The guard bubble to the top of a block, after the combinational operations; 
+- The synchronous updates stay are put in a Guard block. 
+
+This strategy does not work for, for instance, a bypass fifo of length 1 [F]
+(empty in the following example)
+[
+  do old <- fifo_enq_deq F new; 
+  assert (old = new); 
+  A
+]
+
+[
+  t1 <- new; 
+  comb (A) 
+  Guard (t1 = t1 /\ guard (A)) [ fifo 
+ 
+]
+
+*)
+(*
+Inductive update (Phi : state) : list Core.type -> Core.type -> Type :=
+  | register_write : forall t, var Phi (Treg t) -> update Phi (t :: nil) Core.Unit
+  | regfile_write : forall n t (v : var Phi (Tregfile n t)) p, update Phi ([Core.Tlift (Tint p); t])%list Core.Unit. 
+
+Section t. 
+  Variable Var : Core.type -> Type. 
+  Variable Phi : state. 
+  
+  Inductive com := 
+  (* event control *)
+  | Guard : Core.expr Var Core.Bool -> com -> com
+  (* combinational assigmenent *)
+  | Foo : forall t, Core.expr Var t -> (Var t -> com) -> com
+  (* synchronous effect *)
+  | State : forall args res (p : update Phi args res) (exprs : dlist Var args),
+              (Var res -> com) -> com. 
+End t. 
+
+Reserved Notation " c1 '/' st '==>' diff" (at level 40, st at level 39).
+
+ Definition chang (s: Core.state) : state.  
+  eapply List.map . 2: apply s. 
+  intros x. 
+  refine (match x with | Core.Treg t => Treg t | Core.Tvis t => Treg t | Core.Tregfile n t => Tregfile n t end). 
+          Defined.     
+Section eval. 
+  Variable Phi : Core.state. 
+  
+  Definition comp V t (c : Core.action Phi V t ) : com V (chang Phi).
+  refine (match c with 
+              | Core.Return t e => _
+              | Core.Bind t u a f => _
+              | Core.When t e a => _
+              | Core.Primitive args res p exprs  => _
+              | Core.Try a => _
+          end). 
+  admit. 
+  | Try : Core.action Phi Var (Core.Tlift Tunit) ->
+          Core.action Phi Var (Core.Tlift Tunit)
+  induction c. 
+  Definition eval_com  (c : com eval_type Phi) (st : eval_state Phi) (Delta : Diff.T Phi): option (Diff.T Phi). 
+  refine (
+      let fix eval_com (c : com eval_type Phi) :=
+          match c with
+            | Guard g c' => fun st Delta => match eval_expr _ g with 
+                                      | true =>  eval_com c' st Delta 
+                                      | false => Some (Delta)
+                                    end
+            | Foo t e c' => fun st Delta => let v := eval_expr _ e in 
+                                      eval_com (c' v) st Delta
+            | State args res p exprs c' => _
+          end
+      in
+        eval_com c st Delta).  
+  intros st' Delta'. 
+  
+
+refine (match E with true => IHc | false => None end). 
+set (E := c (eval_expr _ e)).
+
+  Inductive com_eval : com -> state -> -> Prop :=
+.  
+  | Eseq : forall st1 st2 st3 c1 c2, 
+             c1 / st1 ==> st2 ->
+             c2 / st2 ==> st3 -> 
+             Cseq c1 c2 / st1 ==> st3
+  | Eset_reg : forall t (v : var regs t) (e : expr t) st1 st2 r, 
+                 eval_expr  st1 e = r ->
+                 update_reg  st1 v r = st2 -> 
+                 (Cset_reg t v e) / st1 ==> st2 
+  | Eset_mem : forall t (v : var mems t) (e : expr t) st1 st2 r, 
+                 eval_expr st1 e = r ->
+                 update_mem st1 v r = st2 -> 
+                 (Cset_mem t v e) / st1 ==> st2
+  | Eifb_true : forall (e : expr Tbool) c1 c2 st1 st2, 
+                  eval_expr  st1 e = true -> 
+                  c1 / st1 ==> st2 ->
+                  (Cifb e c1 c2) / st1 ==> st2
+  | Eifb_false : forall (e : expr Tbool) c1 c2 st1 st2, 
+                   eval_expr st1 e = false -> 
+                   c2 / st1 ==> st2 ->
+                   (Cifb e c1 c2) / st1 ==> st2 
+   where "c1 '/' st '==>' st'" := (com_eval c1 st st').
+
+  
+End t.     
+
+
+(*   Module Diff. 
+    Section t. 
+      Variable Phi : state. 
+      Definition T := eval_env (option ∘ eval_sync) Phi. 
+      Definition add (Delta : T) t (v : var Phi t) w : option T :=
+        match get Phi t v Delta  with 
+          | None =>  Some  (set _ _ Phi t v (Some w) Delta)
+          | Some _ => None 
+        end.
+      
+    End t. 
+    Fixpoint init (Phi : state ): T Phi := 
+      match Phi with 
+        | nil => tt
+        | cons t Phi => (None, init Phi)
+      end. 
+    
+    Fixpoint apply (Phi : state) : T Phi -> eval_env eval_sync Phi -> eval_env eval_sync Phi :=
+      match Phi with 
+        | nil => fun _ _ => tt
+        | cons t Phi => fun Delta E => 
+                       match fst Delta with 
+                         | None => (fst E, apply Phi (snd Delta) (snd E))
+                         | Some d => (d, apply Phi (snd Delta) (snd E))
+                       end
+      end. 
+    
+  End Diff. 
+*)
+Module Sem2.
+  Module Guarded. 
+    (** static semantics: 
+     *)
+    Section t. 
+      Variable Phi : state. 
+      Variable Var : type -> Type. 
+
+          
+      Record  M t := mk_M
+        {
+          content : expr Var t;
+          effects : list effect; 
+          valid : expr Var Bool}. 
+
+      Arguments mk_M {t} _ _ _. 
+      
+      Definition T t := expr Var Bool -> M t. 
+      
+      Definition Return {t} (e : expr Var t) : T t := fun _ => mk_M e nil (#b true).
+
+      Definition Bind {s t} : T s -> (expr Var s -> T t) -> T t.
+      intros x f. 
+      intros Psi. 
+      refine (let x' := x Psi in 
+              let y := f (content _ x') Psi in 
+                mk_M (content _ y) (effects _ x' ++ effects _ y) (valid _ x' && valid _ y )%expr). 
+      Defined. 
+      
+      Definition primitive_denote  args res (p : primitive Phi args res) (exprs : eval_env eval_type args) : T (res). 
+      intros Psi. 
+      destruct p.  
+      (* register read *)
+      
+      (* register write *)
+      (* regfile read *)
+      (* regfile write *)
+
+        match
+          p in (primitive _ l t) return (eval_env eval_type l -> T (eval_type t))
+        with
+          | register_read t v =>
+              fun _ (st : eval_state Phi)
+                  (Delta : Diff.T Phi) => Some (get Phi (Treg t) v st, Delta)
+          | register_write t v =>
+              fun (exprs : eval_env eval_type [t]) (_ : eval_state Phi) (Delta : Diff.T Phi) =>
+                let (w, _) := exprs in
+                  do Delta2 <- Diff.add Phi Delta (Treg t) v w; 
+                  Some (tt, Delta2)
+          | regfile_read n t v p =>
+              fun (exprs : eval_env eval_type [Tlift (W p)]) 
+                  (st : eval_state Phi) (Delta : Diff.T Phi) =>
+                let rf := get Phi (Tregfile n t) v st in
+                let adr := fst exprs in
+                  do v <- Regfile.get rf (Word.unsigned adr); Some (v, Delta)
+          | regfile_write n t v p =>
+              fun (exprs : eval_env eval_type [Tlift (W p); t]) 
+                  (st : eval_state Phi) (Delta : Diff.T Phi) =>
+                let rf := get Phi (Tregfile n t) v st in
+                let rf := match exprs with 
+                              (adr, (w, _)) => Regfile.set rf (Word.unsigned adr) w
+                          end
+                in
+                  do Delta2 <- Diff.add Phi Delta (Tregfile n t) v rf; Some (tt, Delta2)
+        end exprs.
+    End t. 
+  End Dyn. 
+
+  (** dynamic semantics: 
+    - all guard failures are represented by None. 
+    - continuation passing style: the current diff is threaded through the execution 
+  *)
+  Section t. 
+    Variable Phi : state. 
+    Definition eval_action (t : type) (a : action Phi eval_type t) : 
+      (Dyn.T Phi (eval_type t)). 
+
+    refine (
+        let fix eval_action (t : type) (a : action Phi eval_type t) :
+            Dyn.T Phi ( eval_type t) :=
+            match a with
+              | Return t exp => Dyn.Return Phi (eval_expr _ exp)
+              | Bind t u a f => 
+                  let act := eval_action _ a in 
+                    let f' := (fun e => eval_action u (f e)) in 
+                      Dyn.Bind Phi act f'              
+              | When t e a => 
+                  let g1 := eval_expr _ e in 
+                    let a' := eval_action t a in 
+                      match g1 with 
+                        | true => a' 
+                        | false => Dyn.Fail  Phi
+                      end
+              | Primitive args res p exprs => 
+                  Dyn.primitive_denote Phi args res p (dlist_fold' eval_expr _ exprs)
+              | Try a => 
+                  let a := eval_action _ a in 
+                    Dyn.Try Phi a                    
+          end                
+      in  eval_action t a). 
+  Defined.
+  End t. 
+  Arguments eval_action {Phi} {t} _%action _ _.  
+End Sem.           
+
+
+Section s. 
+
+  Variable Phi : state. 
+Section expr. 
+  Variable mems : list type0. 
+  Variable regs : list type0. 
+
+  Inductive expr : type0 -> Type :=
+  | get_reg : forall t, var regs t ->  expr t
+  | get_mem : forall t, var mems t ->  expr t
+  | const : forall (c : constant),  expr (cst_ty c)
+  | op :
+    forall (f : signature), 
+      dlist expr (args f) -> 
+      expr (res f). 
+
+  Inductive com : Type :=
+    | Cskip 
+    | Cseq : com -> com -> com
+    | Cset_reg : forall t (v : var regs t), expr t -> com
+    | Cset_mem : forall t (v : var mems t), expr t -> com
+    | Cifb : expr Tbool -> com  -> com -> com. 
+  
+    
+  Record state :=
+    {
+      st_mems : eval_env eval_type0 mems;
+      st_regs : eval_env eval_type0 regs    
+    }. 
+
+  Reserved Notation " c1 '/' st '==>' st'" (at level 40, st at level 39).
+  Definition eval_expr {t} : state -> expr t -> eval_type0 t. 
+  Admitted. 
+
+  Definition update_reg : forall {t},  state -> var regs t ->  eval_type0 t -> state. Admitted. 
+  Definition update_mem : forall {t},  state -> var mems t -> eval_type0 t -> state. Admitted. 
+  
+  Inductive com_eval : com -> state -> state -> Prop :=
+  | Eskip : forall st, Cskip  / st ==> st
+  | Eseq : forall st1 st2 st3 c1 c2, 
+             c1 / st1 ==> st2 ->
+             c2 / st2 ==> st3 -> 
+             Cseq c1 c2 / st1 ==> st3
+  | Eset_reg : forall t (v : var regs t) (e : expr t) st1 st2 r, 
+                 eval_expr  st1 e = r ->
+                 update_reg  st1 v r = st2 -> 
+                 (Cset_reg t v e) / st1 ==> st2 
+  | Eset_mem : forall t (v : var mems t) (e : expr t) st1 st2 r, 
+                 eval_expr st1 e = r ->
+                 update_mem st1 v r = st2 -> 
+                 (Cset_mem t v e) / st1 ==> st2
+  | Eifb_true : forall (e : expr Tbool) c1 c2 st1 st2, 
+                  eval_expr  st1 e = true -> 
+                  c1 / st1 ==> st2 ->
+                  (Cifb e c1 c2) / st1 ==> st2
+  | Eifb_false : forall (e : expr Tbool) c1 c2 st1 st2, 
+                   eval_expr st1 e = false -> 
+                   c2 / st1 ==> st2 ->
+                   (Cifb e c1 c2) / st1 ==> st2 
+   where "c1 '/' st '==>' st'" := (com_eval c1 st st').
+
+Fixpoint com_denote (c : com) (st1 : state) : option state :=
+  match c with
+    | Cskip => Some st1
+    | Cseq c1 c2 => 
+        do st2 <- com_denote c1 st1;
+        com_denote c2 st2
+    | Cset_reg t v e =>
+        let r := eval_expr st1 e in 
+          Some (update_reg st1 v r)
+    | Cset_mem t v e =>
+        let r := eval_expr st1 e in 
+          Some (update_mem st1 v r)
+    | Cifb e c1 c2  =>
+        let r := eval_expr st1 e in 
+          if r then com_denote c1 st1 
+          else  com_denote c2 st1
+  end. 
+End expr.  
+
+Record RTL :=
+  {
+    mems : list type0;
+    regs : list type0;
+    code : com mems regs; 
+    t_outputs : list type0;
+    outputs : dlist (var regs) t_outputs;
+    t_inputs : list type0;
+    inputs : dlist  (var regs) t_inputs
+  }. 
+
+
+Section semantics. 
+  Variable R : RTL. 
+  
+  Let I := eval_env eval_type0 (t_inputs R). 
+  Let O := eval_env eval_type0 (t_outputs R). 
+
+  Let sigma := state (mems R) (regs R). 
+
+  (* Definition M : Moore.T I O sigma. *)
+  (* constructor.  *)
+  (* Fixpoint zob E F (l : dlist  (var E) F) :  *)
+  (*   eval_env eval_type0 E -> eval_env eval_type0 F := *)
+  (* match l with *)
+  (*   | dlist_nil => fun _ => tt *)
+  (*   | dlist_cons t q T Q => fun X => (get E t T X, zob _ _ Q X) *)
+  (* end.  *)
+  
+  (* intros. eapply zob. apply outputs. apply (st_regs _ _ X).  *)
+  (* intros. apply com_denote. apply (code  R).  *)
+  (* apply X.  *)
+  (* Defined.  *)
+
+End semantics. 
+ (*
+Inductive machine :=
+  {
+    mems : list type0;
+    regs : list type0;
+    instances : list machine;
+    reset : com mems regs ;
+    step : com mems regs
+  }. 
+
+Inductive state (m : machine) := 
+  {
+    ls : local_state (mems m) (regs m);
+    st_machines : dlist _ state (instances m)
+  }.
+  
+Reserved Notation " c1 '/' st '==>' st'" (at level 40, st at level 39).
+
+Inductive com_eval m : com (mems m) (regs m) -> state m -> state m -> Prop :=
+  | Eskip : forall st, Cskip (mems m) (regs m)  / st ==> st
+  | Eseq : forall st1 st2 st3 c1 c2, 
+             c1 / st1 ==> st2 ->
+             c2 / st2 ==> st3 -> 
+             Cseq (mems m) (regs m) c1 c2 / st1 ==> st3
+  | Eset_reg : forall t (v : var (regs m) t) (e : expr (mems m) (regs m) t) st1 st2 r, 
+                 eval_expr _ _ st1 e = r ->
+                 update_reg _ _ st1 r = st2 -> 
+                 (Cset_reg _ _ _ t v e) / st1 ==> st2 (*
+  | Eset_mem : forall t (v : var mems t) (e : expr t) st1 st2 r, 
+                 eval_expr _ st1 e = r ->
+                 update_mem _ st1 r = st2 -> 
+                   (Cset_mem t v e) / st1 ==> st2
+    | Eifb_true : forall (e : expr Tbool) c1 c2 st1 st2, 
+               eval_expr _ st1 e = true -> 
+               c1 / st1 ==> st2 ->
+               (Cifb e c1 c2) / st1 ==> st2
+    | Eifb_false : forall (e : expr Tbool) c1 c2 st1 st2, 
+               eval_expr _ st1 e = false -> 
+               c2 / st1 ==> st2 ->
+               (Cifb e c1 c2) / st1 ==> st2 *)
+    where "c1 '/' st '==>' st'" := (com_eval _ c1 st st').
+ 
+
+
+
+
+
+End expr. 
+  
+
+End expr. 
+Inductive type :=
+| Tregfile : forall (size : nat) (base : type0) , type
+| Tfifo : nat -> type0 -> type
+| Tbase : type0 -> type
+| Tinput  : type0 -> type
+| Toutput : type0 -> type. 
+
+Fixpoint eval_type (t : type) : Type :=
+  match t with
+    | Tregfile size bt =>Regfile.T size (eval_type0 bt) 
+    | Tfifo n bt => FIFO.T n (eval_type0 bt)
+    | Tbase bt => eval_type0 bt
+    | Tinput bt => eval_type0 bt
+    | Toutput bt => eval_type0 bt
+  end. 
+
+Section expr. 
+  Variable Env : list type. 
+  
+  Inductive expr : type0 -> Type :=
+  | Eprim : forall f (args: expr_vector (args (f))), expr ( (res ( f)))
+  | Eget : forall t (v : var Env (Tbase t)), expr t
+  (* operations on arrays *)
+  | Eget_array : forall size  n t (v : var Env (Tregfile size t)), expr (Tint n) -> expr t
+  (* operations on fifo *)
+  | Efirst : forall n t (v : var Env (Tfifo n t)), expr t
+  | Eisfull : forall n t (v : var Env (Tfifo n t)), expr (Tbool)
+  | Eisempty : forall n t (v : var Env (Tfifo n t)), expr (Tbool)
+  (* operations on Inputs *)
+  | Eget_input : forall t (v : var Env (Tinput t)), expr t
+  (* operations on Outputs *)
+  | Eget_output : forall t (v : var Env (Toutput t)), expr t
+                                                      with expr_vector : list type0 -> Type :=
+  | expr_vector_nil : expr_vector nil
+  | expr_vector_cons : forall t q, expr  (t) -> expr_vector q -> expr_vector (t::q). 
+
+
+  Record reg_update (t : type0): Type :=
+    {
+      latch_enable : expr Tbool;
+      data : expr t
+    }. 
+  
+  Record array_update (size : nat) (width : nat) (t : type0) :=
+    {
+      write_addr : expr (Tint width);
+      write_data : expr t;
+      write_enable : expr Tbool
+    }.
+
+  Record fifo_update (t : type0) :=
+    {
+      enqueue_data : expr t;
+      enqueue_enable : expr Tbool;
+      dequeue_enable : expr Tbool;
+      clear_enable : expr Tbool
+    }. 
+  
+  Inductive expr2 : type -> Type :=
+  (* expression to affect and latch enable  *)
+  | Eregister : forall t, reg_update t -> expr2 (Tbase t)
+  (* array operations *)
+  | Earray :  forall size width t, array_update size width t -> 
+                   expr2 (Tregfile size t)
+  (* fifo operations *)
+  | Efifo : forall n t, fifo_update t ->  expr2 (Tfifo n t) 
+  | Enop : forall t, expr2 t. 
+              
+  
+End expr. 
+
+*)*)
